continuing with constructive experiment

ConstructiveSigmaHCOL.v
@@ -84,3 +84,483 @@ Fixpoint SparseUnion {A} {n}:
                   (OptionUnion (Vhead a') (Vhead b') (OptVecComp_hd ok))
                   (SparseUnion (Vtail a') (Vtail b')  (OptVecComp_tl ok))
     end.
+
+Module SigmaHCOL_Operators.
+
+  Global Open Scope nat_scope.
+  
+  Section IndexedOperators.
+
+    (* Returns an element of the vector 'x' which is result of mapping of given
+natrual number by index mapping function f_spec. *)
+    Definition VnthIndexMapped {A:Type}
+               {i o:nat}
+               (x: vector A i)
+               (f: index_map o i)
+               (n:nat) (np: n<o)
+    : A
+      := Vnth x (« f » n np).
+
+    Definition Gather `{Equiv A}
+               {i o: nat}
+               (f: index_map o i)
+               (x: vector A i):
+      vector A o
+      := Vbuild (VnthIndexMapped x f).
+
+    (* Specification of gather as mapping from ouptu to input. NOTE:
+    we are using definitional equality here, as Scatter does not
+    perform any operations on elements of type A *)
+    Lemma Gather_spec `{Equiv A}
+          {i o: nat}
+          (f: index_map o i)
+          (x: vector A i)
+          (y: vector A o):
+      (Gather f x ≡ y) ->  ∀ n (ip : n < o), Vnth y ip ≡ VnthIndexMapped x f n ip.
+    Proof.
+      unfold Gather, Vbuild. 
+      destruct (Vbuild_spec (VnthIndexMapped x f)) as [Vv Vs].
+      simpl.
+      intros.
+      subst.
+      auto.
+    Qed.
+    
+    Lemma Gather_is_endomorphism `{Ae: Equiv A}:
+      ∀ (i o : nat)
+        (x : vector A i),
+      ∀ (f: index_map o i),
+        Vforall (Vin_aux x)
+                (Gather f x).
+    Proof.
+      intros.
+      apply Vforall_eq.
+      intros.
+      unfold Gather in H. 
+      unfold Vin_aux.
+      apply Vbuild_in in H.
+      crush.
+      unfold VnthIndexMapped.
+      apply Vnth_in.
+    Qed.
+
+    Lemma Gather_preserves_P `{Ae: Equiv A}:
+      ∀ (i o : nat) (x : vector A i) (P: A->Prop),
+        Vforall P x
+        → ∀ f : index_map o i,
+          Vforall P (Gather f x).
+    Proof.
+      intros.
+      assert(Vforall (Vin_aux x) (Gather f x))
+        by apply Gather_is_endomorphism.
+      generalize dependent (Gather f x).
+      intros t.
+      rewrite 2!Vforall_eq.
+      crush.
+      assert (Vin_aux x x0) by (apply H0; assumption).
+      rewrite Vforall_eq in H.
+      crush.
+    Qed.
+
+    Lemma Gather_preserves_density `{Ae: Equiv A}:
+      ∀ (i o : nat) (x : svector A i)
+        (f: index_map o i),
+        svector_is_dense x ->
+        svector_is_dense (Gather f x).
+    Proof.
+      intros.
+      unfold svector_is_dense in *.
+      apply Gather_preserves_P.
+      assumption.
+    Qed.
+    
+    Definition VnthInverseIndexMapped {A:Type}
+               {i o:nat}
+               (x: svector A i)
+               (f': partial_index_map o i)
+               (n:nat) (np: n<o)
+      : option A
+      :=
+        let f := partial_index_f _ _ f' in
+        let f_spec := partial_index_f_spec _ _  f' in
+        match (f n) as fn return f n ≡ fn -> option A with        
+        | None => fun _ => None
+        | Some z => fun p => Vnth x (f_spec n np z p)
+        end eq_refl.
+    
+    Program Definition Scatter {A:Type}
+            {i o: nat}
+            (f: index_map i o)
+            (x: svector A i) : svector A o
+      :=
+        Vbuild (fun n np =>
+                  VnthInverseIndexMapped x (build_inverse_index_map f) n np).
+
+    (* Specification of scatter as mapping from input to output. NOTE:
+    we are using definitional equality here, as Scatter does not
+    perform any operations on elements of type A *)
+    Lemma Scatter_spec `{Equiv A}
+          {i o: nat}
+          (f: index_map i o)
+          (x: svector A i)
+          (y : svector A o):
+      index_map_injective f -> (Scatter f x ≡ y) ->  ∀ n (ip : n < i), Vnth x ip ≡ VnthIndexMapped y f n ip.
+    Proof.
+      intros J S n ip.
+      unfold VnthIndexMapped.
+      unfold Scatter in S.
+      subst y.
+      rewrite Vbuild_nth.
+      assert(L: partial_index_f o i (build_inverse_index_map f) (⟦f ⟧ n) ≡ Some n).
+      {
+        apply build_inverse_index_map_is_left_inverse; try assumption.
+        reflexivity.
+      }
+
+      (* At this point 'rewrite L' should work but it does not, so we will generalize the hell out of it, and remove unnecessary hypothesis to work around this problem *)
+      
+      remember (build_inverse_index_map f) as f' eqn:F.
+      unfold VnthInverseIndexMapped.
+
+      generalize (partial_index_f_spec o i f' (⟦f ⟧ n) («f » n ip));  intros l.
+      destruct (partial_index_f o i f' (⟦f ⟧ n)).
+      inversion L.
+      subst n0.
+      generalize (l n eq_refl); intros l0.
+      replace l0 with ip by apply proof_irrelevance.
+      reflexivity.
+      congruence.
+    Qed.
+    
+    (* Specification of scatter as mapping from output to input.
+    NOTE: we are using definitional equality here, as Scatter does not
+    perform any operations on elements of type A *)
+    Lemma Scatter_rev_spec `{Equiv A}:
+    forall 
+          {i o: nat}
+          (f: index_map i o)
+          (x: svector A i)
+          (y : svector A o),
+      (Scatter f x ≡ y) ->  (∀ n (ip : n < o), Vnth y ip ≡ VnthInverseIndexMapped x (build_inverse_index_map f) n ip).
+    Proof.
+      intros i o f x y.
+      unfold Scatter, Vbuild. 
+      destruct (Vbuild_spec
+                  (λ (n : nat) (np : n < o),
+       VnthInverseIndexMapped x (build_inverse_index_map f) n np)) as [Vv Vs].
+      simpl.
+      intros.
+      subst.
+      auto.
+    Qed.
+
+  End IndexedOperators.
+
+  Definition GathH `{Equiv A}
+             (i o base stride: nat)
+             {range_bound: (base+(pred o)*stride) < i}
+             {snz: stride ≢ 0} 
+    :
+      (svector A i) -> svector A o
+    :=
+      Gather 
+        (@h_index_map o i base stride range_bound snz).
+
+  Definition ScatH `{Equiv A}
+             (i o base stride: nat)
+             {domain_bound: (base+(pred i)*stride) < o}
+             {snz: stride ≢ 0} 
+    :
+      (svector A i) -> svector A o
+    :=
+      Scatter 
+        (@h_index_map i o base stride domain_bound snz).
+  
+End SigmaHCOL_Operators.
+
+Import SigmaHCOL_Operators.
+
+Section SigmaHCOL_Language.
+  (* Sigma-HCOL language, introducing even higher level concepts like variables *)
+
+  Context {A:Type} {Ae: Equiv A}.
+  
+  Inductive varname : Type :=
+    Var : string → varname.
+  
+  Theorem eq_varname_dec: forall id1 id2 : varname, {id1 ≡ id2} + {id1 ≢ id2}.
+  Proof.
+    intros id1 id2.
+    destruct id1 as [n1]. destruct id2 as [n2].
+    destruct (string_dec n1 n2) as [Heq | Hneq].
+    left. rewrite Heq. reflexivity.
+    right. intros contra. inversion contra. apply Hneq.
+    assumption.
+  Qed.
+  
+  Inductive aexp : Set :=
+  | AConst : nat → aexp
+  | AValue : varname → aexp
+  | APlus : aexp → aexp → aexp
+  | AMinus : aexp → aexp → aexp
+  | AMult : aexp → aexp → aexp.
+  
+  Inductive SOperator: nat -> nat -> Type :=
+  (* --- HCOL basic operators --- *)
+  | SHOScatH {i o} (base stride:aexp): SOperator i o
+  | SHOGathH {i o} (base stride: aexp): SOperator i o
+  (* TODO: proper migh not neccessary be part of SOperator as it only needed for rewriting *)
+  | SHOBinOp o (f:A->A->A) `{pF: !Proper ((=) ==> (=) ==> (=)) f}: SOperator (o+o) o
+  (* Lifted generic HCOL operator *)
+  | SOHCOL {i} {o} (h:HOperator i o): SOperator i o
+  (* --- Copies of HCOL operators which can use variabeles --- *)
+  | SHOInfinityNorm {i}: SOperator i 1
+  | SOReduction i (f: A->A->A) `{pF: !Proper ((=) ==> (=) ==> (=)) f} (idv:A): SOperator i 1
+  (* TODO:
+  | HOPointWise2 o (f:A->A->A) `{pF: !Proper ((=) ==> (=) ==> (=)) f}: HOperator (o+o) o
+  | HOInduction n (f:A->A->A) `{pF: !Proper ((=) ==> (=) ==> (=)) f} (initial:A): HOperator 1 n
+  | HOCross i1 o1 i2 o2:  HOperator i1 o1 -> HOperator i2 o2 -> HOperator (i1+i2) (o1+o2)
+  | HOTLess i1 i2 o: HOperator i1 o -> HOperator i2 o -> HOperator (i1+i2) o
+  | HOStack i o1 o2: HOperator i o1 -> HOperator i o2 -> HOperator i (o1+o2)
+   *)
+  (* --- HCOL compositional operators --- *)
+  | SHOCompose i {t} o: SOperator t o -> SOperator i t -> SOperator i o
+  (* NOTE: dimensionality of the body must match that of enclosing ISUMUnion. *)
+  | SHOISumUnion {i o} (var:varname) (r:aexp): SOperator i o -> SOperator i o
+  .
+  
+  Definition state := varname -> nat.
+  
+  Definition empty_state: state :=
+    fun x => 0.
+  
+  Definition update (st : state) (x : varname) (n : nat) : state :=
+    fun x' => if eq_varname_dec x x' then n else st x'.
+  
+  Fixpoint evalAexp (st:state) (e:aexp): nat :=
+    match e  with
+    | AConst x => x
+    | AValue x => st x
+    | APlus a b => Peano.plus (evalAexp st a) (evalAexp st b) 
+    | AMinus a b => Peano.minus (evalAexp st a) (evalAexp st b) 
+    | AMult a b => Peano.mult (evalAexp st a) (evalAexp st b) 
+    end.
+
+  Lemma update_apply:
+    ∀ (var : varname) (st : state) (x:nat),
+      (update st var x var) ≡ x.
+  Proof.
+    intros var st x.
+    compute.
+    break_if.
+    reflexivity.
+    congruence.
+  Qed.
+
+  Lemma update_eval:
+    ∀ (var : varname) (st : state) (x:nat),
+      evalAexp (update st var x) (AValue var) ≡ x.
+  Proof.
+    intros.
+    simpl.
+    apply update_apply.
+  Qed.
+
+  Fixpoint varFreeIn (v:varname) (e: aexp) : Prop
+    :=
+      match e with
+      | AConst _ => True
+      | AValue x => x<>v
+      | APlus a b => varFreeIn v a /\ varFreeIn v b
+      | AMinus a b => varFreeIn v a /\ varFreeIn v b
+      | AMult a b => varFreeIn v a /\ varFreeIn v b
+      end.
+  
+  Lemma eval_update_free:
+    ∀ (v: varname) (exp:aexp) (st : state) (x:nat),
+      varFreeIn v exp ->
+      evalAexp (update st v x) exp ≡ evalAexp st exp.
+  Proof.
+    Local Ltac uniop_case F :=
+      (unfold varFreeIn in F;
+       unfold update; simpl;
+       destruct eq_varname_dec; congruence).
+    
+    Local Ltac binop_case F H1 H2:=
+      (simpl in F; decompose [and] F; clear F;
+       unfold evalAexp; fold evalAexp;
+       rewrite H1, H2; 
+       [reflexivity | assumption| assumption]).
+    
+    intros v exp st x F.
+    induction exp;
+      solve [ auto | uniop_case F | binop_case F IHexp1 IHexp2].
+  Qed.
+  
+  Section SigmaHCOL_Eval.
+    Context    
+      `{Az: Zero A} `{A1: One A}
+      `{Aplus: Plus A} `{Amult: Mult A} 
+      `{Aneg: Negate A}
+      `{Ale: Le A}
+      `{Alt: Lt A}
+      `{Ato: !@TotalOrder A Ae Ale}
+      `{Aabs: !@Abs A Ae Ale Az Aneg}
+      `{Asetoid: !@Setoid A Ae}
+      `{Aledec: !∀ x y: A, Decision (x ≤ y)}
+      `{Aeqdec: !∀ x y, Decision (x = y)}
+      `{Altdec: !∀ x y: A, Decision (lt x y)}
+      `{Ar: !Ring A}
+      `{ASRO: !@SemiRingOrder A Ae Aplus Amult Az A1 Ale}
+      `{ASSO: !@StrictSetoidOrder A Ae Alt}.
+
+    Definition evalScatH
+               {i o: nat}
+               (st:state)
+               (base stride:aexp)
+               (snz: evalAexp st stride ≢ 0)
+               (domain_bound: (evalAexp st base) + pred i * (evalAexp st stride) < o)
+               (v:svector A i):
+      @svector A o :=
+      ScatH
+        (snz:=snz)
+        (domain_bound:=domain_bound)
+        i o (evalAexp st base) (evalAexp st stride) v.
+
+    Definition evalGathH
+               {i o: nat}
+               (st:state)
+               (base stride:aexp)
+               (snz: evalAexp st stride ≢ 0)
+               (range_bound: (evalAexp st base) + pred o * (evalAexp st stride) < i)
+               (v: svector A i):  svector A o :=
+      GathH
+        (snz:=snz)
+        (range_bound:=range_bound)
+        i o (evalAexp st base) (evalAexp st stride) v.
+    
+    (* TODO: move *)
+    Fixpoint vector_from_svector {A} `{Zero A}  {n} (v:svector A n): vector A n :=
+      Vmap (fun x => match x with
+                  | None => zero
+                  | Some v => v
+                  end) v.
+
+    (* TODO: just use evalHOperator *)
+    Definition evalBinOp
+               {o: nat}
+               (f: A->A->A) `{pF: !Proper ((=) ==> (=) ==> (=)) f}
+               (v: svector A (o+o)):
+      svector A o :=
+      (svector_from_vector
+         ∘ evalHCOL (HOPointWise2 o f (Ae:=Ae) (pF:=pF))
+         ∘ vector_from_svector
+      ) v.
+
+    (* TODO: just use evalHOperator *)
+    Definition evalInfinityNorm
+               {i: nat}
+               (st:state)
+               (v: svector A i):
+      svector A 1 :=
+      (svector_from_vector
+         ∘ evalHCOL (HOInfinityNorm)
+         ∘ vector_from_svector
+      ) v.
+
+    (* TODO: just use evalHOperator *)
+    Definition evalReduction
+               {i: nat}
+               (st:state)
+               (f: A->A->A) `{pF: !Proper ((=) ==> (=) ==> (=)) f}
+               (idv:A)
+               (v: svector A i):
+      svector A 1 :=
+      (svector_from_vector
+         ∘ evalHCOL (HOReduction i f idv)
+         ∘ vector_from_svector
+      ) v.
+
+    Definition evalHOperator
+               {i o: nat}
+               (h: HOperator i o)
+               (v: svector A i):
+      svector A o :=
+      (svector_from_vector
+         ∘ evalHCOL h
+         ∘ vector_from_svector
+      ) v.
+
+
+    (*TODO: need {rnz: evalAexp st r ≢ 0} *)
+    Fixpoint evalSigmaHCOL
+             {i o: nat}
+             (st:state)
+             (op: SOperator i o)
+             (v:svector A i): svector A o
+      :=
+        (match op in @SOperator i o return svector A i -> svector A o
+         with
+         | SHOISumUnion i o var r body as su =>
+           (fun v0 => 
+              match (evalAexp st r)
+              with
+              | O => Error "Invalid SHOISumUnion range"
+              | (S p) =>
+                Vfold_left (@ErrSparseUnion A o)
+                           (OK (empty_svector o))
+                           (Vbuild 
+                              (fix en (n':nat) (np:n'<S p) := evalSigmaHCOL (update st var n') body v0))
+              end
+           )
+         | SHOCompose _ _ _ f g  =>
+           (fun v0 =>
+              match evalSigmaHCOL st g v0 with
+              | Error msg => Error msg
+              | OK gv => evalSigmaHCOL st f gv
+              end)
+         | SHOScatH _ _ base stride => evalScatH st base stride
+         | SHOGathH _ _ base stride => evalGathH st base stride
+         | SHOBinOp _ f _ => evalBinOp f
+         | SOHCOL _ _ h => evalHOperator h
+         | SHOInfinityNorm _ => evalInfinityNorm st
+         | SOReduction _ f pf idv => evalReduction st f idv
+         end) v.
+    
+        
+    Global Instance SigmaHCOL_equiv {i o:nat}: Equiv (SOperator i o) :=
+      fun f g => forall st (x:svector A i), evalSigmaHCOL st f x = evalSigmaHCOL st g x.
+
+    Lemma SigmaHCOL_extensionality {i o} (f g : SOperator i o) :
+      (forall v st, evalSigmaHCOL st f v = evalSigmaHCOL st g v) -> f = g.
+    Proof.
+      intros.
+      unfold equiv, SigmaHCOL_equiv.
+      auto.
+    Qed.
+
+    Global Instance SigmaHCOL_Equivalence {i o:nat}
+           `{!Equivalence (@equiv A _)}
+      : Equivalence (@SigmaHCOL_equiv i o).
+    Proof.
+      unfold SigmaHCOL_equiv.
+      constructor.
+      unfold Reflexive. intros. apply SigmaHCOL_extensionality. intros. reflexivity.
+      unfold Symmetric. intros. apply SigmaHCOL_extensionality. intros. symmetry. auto.
+      unfold Transitive. intros. apply SigmaHCOL_extensionality. intros. rewrite H. auto.
+    Qed.
+    
+    Global Instance SigmaHCOL_Setoid {i o}: Setoid (SOperator i o).
+    Proof.
+      unfold Setoid.
+      apply SigmaHCOL_Equivalence.
+    Qed.
+    
+  End SigmaHCOL_Eval.
+End SigmaHCOL_Language.
+
+
+
+
+
+
